Bryant Har

### Q1
###### Part A
Set origin to be (0,0). Then, 
$U = mgy_m = mg(l-l\cos(\theta))$
We also find kinetic energy, using the image
$$(x_m, y_m)= (l\sin(\theta), l-l\cos(\theta)) \implies (\dot x_m, \dot y_m)= (l\cos(\theta), l\sin(\theta)) \dot \theta$$
$$\implies v=l\dot \theta$$
$T=\frac{1}{2}ml^2\dot \theta^2$
The lagrangian, then, is
$$\implies L = T-U=\boxed{L=\frac{1}{2}ml^2\dot \theta^2-mg(l-l\cos(\theta))}$$
###### Part B
$$\mathcal{L}=\frac{dL}{d\theta}-\frac{d}{dt}\frac{dL}{d \dot\theta}$$
Substituting L,
$$\mathcal{L}=0=\frac{dL}{d\theta}-\frac{d}{dt}\frac{dL}{d \dot\theta}=-mgl\sin(\theta)-ml^2\ddot \theta$$
We rearrange terms to arrive at our final EL equation,
$$\boxed{ml^2\ddot \theta=-
mgl\sin(\theta)}$$
Alternatively,    $l\ddot \theta=-g\sin(\theta)$

###### Part C


### Q2
###### Part a
