### Qa
Following example 10.7 from the book, we can take the laplace transform and generate these conditions,
$$M\ddot x+kx = \delta(t)$$$$M\mathcal{L}(\ddot x)+k\mathcal{L}(x) = \mathcal{L}(\delta(t))$$
Per the book, we have the choice to use the $t=0^-$ approach definition for our Laplace transform. Of course, by causality, everything is at rest,
$$M(s^2X-sx(0^-)-\dot x(0^-))+kX = 1$$
$$Ms^2X+kX = 1$$
$$\omega^2 = \frac{K}{M} \implies X = \frac{1/M}{s^2+\omega^2}$$
By residue theorem, we take the inverse transform. We've done this many times already and should already know this is sinusoidal. The sum of the residue are clearly,
$$x= \frac{1}{M}\frac{1}{2i\omega}\big[e^{i\omega t}-e^{-i\omega t} \big]$$
$$x= \frac{1}{M\omega}\sin(\omega t),\ \ \ t>0$$
$$\dot x= \frac{1}{M}\cos(\omega t),\ \ \ t>0$$
$$\ddot x= -\frac{\omega}{M}\sin(\omega t),\ \ \ t>0$$
Then, by inspection of this solution for $x$, the initial conditions are trivially found to be
$$\boxed{\begin{cases}x(0)=\ddot x(0) = 0,\ \ \ \\\dot x(0) = \frac{1}
{M}\end{cases}}$$
Where as always, $\omega^2 = K/M$.
### Qb
We find the initial conditions imposed similarly,
$$M\mathcal{L}(\ddot x)+k\mathcal{L}(x) = \mathcal{L}(\delta'(t))$$
$$M(s^2X-sx(0^-)-\dot x(0^-))+kX = s\mathcal{L}(\delta(0^-))-\delta(0^-)$$
$$Ms^2X+kX = s$$
$$X = \frac{s/M}{s^2+\omega^2}$$
By residue theorem, we take the inverse transform. We've done this many times already and should already know this is sinusoidal. The sum of the residue are clearly,
$$x= \frac{1}{M}\frac{\omega i}{2i\omega}\big[e^{i\omega t}+e^{-i\omega t} \big]$$
For $t>0$,
$$x= \frac{1}{M}\cos(\omega t)$$
$$\dot x= -\frac{\omega}{M}\sin(\omega t)$$
$$\ddot x= -\frac{\omega^2}{M}\cos(\omega t)$$
To make this true, we look at the solution and derivatives and trivially see that
$$\boxed{x(0)=\frac{1}{M},\ \dot x(0) = 0,\ \ddot x(0) = -\frac{\omega^2}{M}}$$
Where as always, $\omega^2 = K/M$.
### Qc
We use a similar approach,
$$M\ddot x+kx = \delta(t)+te^{-t},\ \ \ t\geq0$$$$M\mathcal{L}(\ddot x)+k\mathcal{L}(x) = \mathcal{L}(\delta(t)+te^{-t})$$
Per the book, we have the choice to use the $t=0^-$ approach definition for our Laplace transform. Of course, by causality, everything is at rest. We take the laplace transform of the exponential as well,
$$M(s^2X-sx(0^-)-\dot x(0^-))+kX = 1
+\int_{0}^{\infty}dt\ te^{-t}e^{-st}=1+\dfrac{1}{\left(s+1\right)^2}$$
$$(s^2+\omega^2) X = \frac{1}{M}+\dfrac{1}{M\left(s+1\right)^2}$$
$$X = \frac{1}{M(s^2+\omega^2)}+\dfrac{1}{M\left(s+1\right)^2(s^2+\omega^2)}$$
We already know 
$$\mathcal{L^{-1}}(\frac{1}{M(s^2+\omega^2)})=\frac{1}{M\omega}\sin(\omega t),\ \ \ t>0$$
We use partial fractions and residue theorem. By partial fractions calculator and laplace table, we arrive at,
$$\mathcal{L^{-1}}\bigg(\dfrac{1}{M\left(s+1\right)^2(s^2+\omega^2)}\bigg) = 

\frac{1}{M}\bigg[\frac{te^{-t}}{1+\omega^2}+\frac{2e^{-t}}{(1+\omega^2)^2}+\frac{-2\omega\cos(\omega t)+\sin(\omega t)-\omega^2\sin(\omega t)}{\omega(1+\omega^2)^2}\bigg]$$
Collecting our results,
$$\mathcal{L^{-1}}(X) = x= 

\frac{1}{M}\bigg[\frac{1}{\omega}\sin(\omega t)+\frac{te^{-t}}{1+\omega^2}+\frac{2e^{-t}}{(1+\omega^2)^2}+\frac{-2\omega\cos(\omega t)+\sin(\omega t)-\omega^2\sin(\omega t)}{\omega(1+\omega^2)^2}\bigg]$$
We find our final expression for $x$ and $\dot x$ (differentiating above expression by calculator),
$$\boxed{ x = \begin{cases}

\frac{1}{M}\bigg[\frac{\sin(\omega t)}{\omega}+\frac{te^{-t}}{1+\omega^2}+\frac{2e^{-t}}{(1+\omega^2)^2}-\frac{2\omega\cos(\omega t)+\sin(\omega t)-\omega^2\sin(\omega t)}{\omega(1+\omega^2)^2}\bigg]
\ \ \  t\geq0\\
\ \ \ \ \ \ \ \ \ \ \ \ \ \ \ \ \ \ \ \ \ \ \ \ \ \ \ \ \ \ \ \ \ \ \ \ \ \ \ \ \ \ \ \ \ \ \ \ \ \ \ \ 0 \ \ \ \ \ \ \ \ \ \ \ \ \ \ \ \ \ \ \ \ \ \ \ \ \ \ \ \  \ \ \ \ \ \ \ \ \ \ \ \ \ \ \ \ \ \ \ \ \ \ \ \ \ t<0
\end{cases}}$$
$$\boxed{\dot x = \begin{cases}

\frac{1}{M}\bigg[\frac{2{\omega}^2\sin\left({\omega}t\right)+{\omega}^3\cos\left({\omega}t\right)-{\omega}\cos\left({\omega}t\right)}{{\omega}\cdot\left({\omega}^2+1\right)^2}+\cos\left({\omega}t\right)-\frac{t\mathrm{e}^{-t}}{{\omega}^2+1}+\frac{\mathrm{e}^{-t}}{{\omega}^2+1}-\frac{2\mathrm{e}^{-t}}{\left({\omega}^2+1\right)^2}\bigg]\ \ \  t\geq0\\
\ \ \ \ \ \ \ \ \ \ \ \ \ \ \ \ \ \ \ \ \ \ \ \ \ \ \ \ \ \ \ \ \ \ \ \ \ \ \ \ \ \ \ \ \ \ \ \ \ \ \ \ 0 \ \ \ \ \ \ \ \ \ \ \ \ \ \ \ \ \ \ \ \ \ \ \ \ \ \ \ \  \ \ \ \ \ \ \ \ \ \ \ \ \ \ \ \ \ \ \ \ \ \ \ \ \ t<0
\end{cases}}$$
Where as always, $\omega^2 = K/M$.
